Progress on a new version of Blake2b incremental

code/blake2b/experimental/Hacl.Impl.Blake2b.Incremental.fst
@@ -24,26 +24,48 @@ module SpecI = Spec.Blake2.Incremental
 #set-options "--z3rlimit 200 --max_fuel 0"
 
 
+let n_t = size_t
+let n_tp = lbuffer n_t 1ul
+
+let pl_t = l:size_t{v l <= v size_block}
+let pl_tp = lbuffer pl_t 1ul
+
+
 (** Define the state *)
 noeq type state_r = {
   hash: hash_wp;
-  n: size_t;
-  pl: l:size_t{v l <= v size_block};
+  n: n_tp;
+  pl: pl_tp;
   block: block_p;
 }
 
 
 unfold let state_inv (h:mem) (state:state_r) =
-  live h state.hash /\ live h state.block /\ disjoint state.hash state.block
+  live h state.hash /\ live h state.block
+  /\ live h state.n /\ live h state.pl
+  /\ disjoint state.hash state.block
+  /\ disjoint state.hash state.n
+  /\ disjoint state.hash state.pl
+  /\ disjoint state.block state.pl
+  /\ disjoint state.block state.n
+  /\ disjoint state.n state.pl
 
-unfold let state_inv_trans (state0:state_r) (state1:state_r) =
-  state0.hash == state1.hash /\ state0.block == state1.block
+
+(* unfold let state_inv_trans (state0:state_r) (state1:state_r) = *)
+(*   state0.hash == state1.hash *)
+(*   /\ state0.block == state1.block *)
+(*   /\ state0.n == state1.n *)
+(*   /\ state0.pl == state1.pl *)
 
 unfold let state_empty (h:mem) (state:state_r) =
   h.[|state.hash|] == Seq.create Spec.size_hash_w (u64 0) /\
-  v state.n == 0 /\
-  v state.pl == 0 /\
+  h.[|state.n|] == Seq.create 1 (size 0) /\
+  h.[|state.pl|] == Seq.create 1 (size 0) /\
   h.[|state.block|] == Seq.create (Spec.size_block Spec.Blake2B) (u8 0)
+
+
+(* unfold let state_modifies4 (state:state_r) (h0:mem) (h1:mem) = *)
+(*   modifies4 state.hash state.block state.n state.pl h0 h1 *)
 
 val state_hash_eq: h:mem -> state_r -> (SpecI.state_r Spec.Blake2B) -> prop
 let state_hash_eq h istate sstate =
@@ -56,18 +78,36 @@ let state_block_eq h istate sstate =
 val state_eq: h:mem -> state_r -> (SpecI.state_r Spec.Blake2B) -> prop
 let state_eq h istate sstate =
   sstate.SpecI.hash == h.[|istate.hash|] /\
-  sstate.SpecI.n == v istate.n /\
-  sstate.SpecI.pl == v istate.pl /\
+  sstate.SpecI.n == v (Lib.Sequence.index h.[|istate.n|] 0) /\
+  sstate.SpecI.pl == v (Lib.Sequence.index h.[|istate.pl|] 0) /\
   sstate.SpecI.block == h.[|istate.block|]
 
 
 val spec_of: h:mem -> state_r -> GTot (SpecI.state_r Spec.Blake2B)
 let spec_of h state =
   let hash: Spec.hash_ws Spec.Blake2B = h.[|state.hash|] in
-  let n: size_nat = v state.n in
-  let pl: l:size_nat{l <= Spec.size_block Spec.Blake2B} = v state.pl in
+  let n: size_nat = v (Lib.Sequence.index h.[|state.n|] 0) in
+  let pl: l:size_nat{l <= Spec.size_block Spec.Blake2B} =  v (Lib.Sequence.index h.[|state.pl|] 0) in
   let block: Spec.block_s Spec.Blake2B = h.[|state.block|] in
   Spec.Blake2.Incremental.Mkstate_r hash n pl block
+
+val gstate_get_n: h:mem -> state:state_r -> GTot (n:n_t{v n == (spec_of h state).SpecI.n})
+let gstate_get_n h state = Lib.Sequence.index (as_seq h state.n) 0
+
+val state_get_n: state:state_r -> Stack n_t
+  (requires fun h -> state_inv h state)
+  (ensures fun h0 n h1 -> h0 == h1 /\ v n == v (gstate_get_n h0 state))
+  (* (ensures fun h0 n h1 -> v n == (spec_of h0 state).SpecI.n) *)
+let state_get_n state = index state.n 0ul
+
+
+val gstate_get_pl: h:mem -> state:state_r -> GTot (n:n_t{v n == (spec_of h state).SpecI.pl})
+let gstate_get_pl h state = Lib.Sequence.index (as_seq h state.pl) 0
+
+val state_get_pl: state:state_r -> Stack pl_t
+  (requires fun h -> state_inv h state)
+  (ensures fun h0 pl h1 -> h0 == h1 /\ v pl == v (gstate_get_pl h0 state))
+let state_get_pl state = index state.pl 0ul
 
 
 val blake2b_incremental_init:
@@ -75,21 +115,20 @@ val blake2b_incremental_init:
   -> kk: size_t{v kk <= 64}
   -> k: lbuffer uint8 kk
   -> nn: size_t{1 <= v nn /\ v nn <= 64} ->
-  Stack state_r
+  Stack unit
   (requires fun h ->
     live h state.hash /\ live h k /\
     disjoint state.hash k /\
     state_inv h state /\
     state_empty h state)
-  (ensures  fun h0 rstate h1 ->
-    modifies1 state.hash h0 h1 /\
-    spec_of h1 rstate == SpecI.blake2_incremental_init Spec.Blake2B h0.[|k|] (v nn))
+  (ensures  fun h0 _ h1 ->
+    modifies2 state.hash state.n h0 h1 /\
+    spec_of h1 state == SpecI.blake2_incremental_init Spec.Blake2B h0.[|k|] (v nn))
 
 let blake2b_incremental_init state kk k nn =
   blake2b_init state.hash kk k nn;
-  let n = if kk =. 0ul then 0ul else 1ul in
-  let rstate = { state with n = n; } in
-  rstate
+  let n: n_t = if kk =. 0ul then 0ul else 1ul in
+  upd state.n 0ul n
 
 
 noextract
@@ -160,37 +199,35 @@ let spec_blake2_incremental_update_loop init blocks hash =
     ) hash
 
 
-
 val blake2b_incremental_update_loop:
     state:state_r
   -> n:size_t
   -> blocks:lbuffer uint8 (n *. size_block) ->
   Stack unit
   (requires fun h ->
-    state_inv h state /\ live h blocks /\
+    live h blocks /\
     disjoint state.hash blocks /\ disjoint state.block blocks /\
     state_inv h state /\
-    v n * v size_block <= max_size_t /\
-    v ((state.n +. n) *. size_block) <= pow2 128 - 1)
+    v n * v size_block <= max_size_t)
+//    /\ v ((state.n +. n) *. size_block) <= pow2 128 - 1)
   (ensures  fun h0 _ h1 ->
     modifies1 state.hash h0 h1
-    /\ h1.[|state.hash|] == spec_blake2_incremental_update_loop (v state.n) h0.[|blocks|] h0.[|state.hash|])
+    /\ h1.[|state.hash|] == spec_blake2_incremental_update_loop (v (Lib.Sequence.index h0.[|state.n|] 0)) h0.[|blocks|] h0.[|state.hash|])
 
 let blake2b_incremental_update_loop state n blocks =
   admit();
   let h0 = ST.get () in
   [@inline_let]
-  let spec h = spec_incremental_update_block (v state.n) (v n) (v n * Spec.size_block Spec.Blake2B) h.[|blocks|] in
+  let spec h = spec_incremental_update_block (v (Lib.Sequence.index h0.[|state.n|] 0)) (v n) (v n * Spec.size_block Spec.Blake2B) h.[|blocks|] in
   loop1 h0 n state.hash spec
   (fun i ->
     Loops.unfold_repeati (v n) (spec h0) h0.[|state.hash|] (v i);
     let block = sub blocks (i *. size_block) size_block in
-    let n64 = to_u64 state.n in
+    let n64 = to_u64 (state_get_n state) in
     let i64 = to_u64 i in
     let size_block64 = to_u64 size_block in
     let prev = to_u128 ((n64 +! i64 +! (u64 1)) *! size_block64) in
     blake2b_update_block state.hash prev block)
-
 
 
 noextract
@@ -242,7 +279,7 @@ let spec_compute_prev n =
 
 
 val compute_prev:
-  n:size_t ->
+  n:n_t ->
   Tot (r:uint128{v r == v (spec_compute_prev (v n))})
 
 let compute_prev n  =
@@ -265,35 +302,39 @@ val spec_blake2b_incremental_update_inner_longer1:
 noextract
 let spec_blake2b_incremental_update_inner_longer1 ll input state rb ll0 =
   let open Spec.Blake2.Incremental in
-  let tlen = v (spec_compute_prev state.SpecI.n) in
+  let n = state.SpecI.n in
+  let tlen = v (spec_compute_prev n) in
   let hash = Spec.blake2_update_block Spec.Blake2B tlen state.SpecI.block state.SpecI.hash in
-  let state = {state with hash = hash; n = state.SpecI.n + 1; pl = 0;} in
+  let state = {state with hash = hash; n = n + 1; pl = 0;} in
   state
 
 
 inline_for_extraction
 val blake2b_incremental_update_inner_longer1:
-    state:state_r
-  -> ll:size_t{v state.n + 1 + (v ll / v size_block) <= max_size_t}
+    #h:mem
+  -> state:state_r
+  -> ll:size_t{v (gstate_get_n h state) + 1 + (v ll / v size_block) <= max_size_t}
   -> input:lbuffer uint8 ll
   -> rb:size_t{v rb <= v size_block}
   -> ll0:size_t{v ll0 = (if ll <. rb then v ll else v rb)} ->
-  Stack state_r
+  Stack unit
   (requires fun h ->
     state_inv h state /\ live h input /\
     disjoint state.hash input /\ disjoint state.block input /\
     state_inv h state /\
-    v (state.n *. size_block) + v ll < pow2 128)
-  (ensures  fun h0 rstate h1 ->
-    modifies2 state.hash state.block h0 h1 /\
-    state_inv h1 rstate /\
-    state_inv_trans state rstate /\
-    state_eq h1 rstate (spec_blake2b_incremental_update_inner_longer1 (v ll) h0.[|input|] (spec_of h0 state) (v rb) (v ll0)))
+    (spec_of h state).SpecI.n + 1 <= max_size_t /\
+    (v (gstate_get_n h state) * v size_block) + v ll < pow2 128)
+  (ensures  fun h0 _ h1 ->
+    modifies3 state.hash state.n state.pl h0 h1 /\
+    state_eq h1 state (spec_blake2b_incremental_update_inner_longer1 (v ll) h0.[|input|] (spec_of h0 state) (v rb) (v ll0)))
 
-let blake2b_incremental_update_inner_longer1 state ll input rb ll0 =
-  let tlen = compute_prev state.n in
+let blake2b_incremental_update_inner_longer1 #h state ll input rb ll0 =
+  let n: n_t = state_get_n state in
+  let tlen = compute_prev n in
   blake2b_update_block state.hash tlen state.block;
-  {state with n = state.n +! 1ul; pl = 0ul}
+  upd state.n 0ul (n +! 1ul);
+  upd state.pl 0ul 0ul
+//  {state with n = state.n +! 1ul; pl = 0ul}
 
 
 noextract
@@ -317,28 +358,30 @@ let spec_blake2b_incremental_update_inner_longer2 ll input state rb ll0 =
 
 inline_for_extraction
 val blake2b_incremental_update_inner_longer2:
-    state:state_r
+    #h:mem
+  -> state:state_r
   -> ll:size_t
   -> input:lbuffer uint8 ll
   -> rb:size_t{v rb <= v size_block}
-  -> ll0:size_t{v ll0 = (if ll <. rb then v ll else v rb) /\ v state.n + (v ll - v ll0) / v size_block <= max_size_t} ->
-  Stack state_r
+  -> ll0:size_t{v ll0 = (if ll <. rb then v ll else v rb)} ->
+  Stack unit
   (requires fun h ->
     state_inv h state /\ live h input /\
     disjoint state.hash input /\ disjoint state.block input /\
-    v (state.n *. size_block) + v ll < pow2 128)
-  (ensures  fun h0 rstate h1 ->
-    modifies2 state.hash state.block h0 h1 /\
-    state_inv h1 rstate /\
-    state_inv_trans state rstate /\
-    state_eq h1 rstate (spec_blake2b_incremental_update_inner_longer2 (v ll) h0.[|input|] (spec_of h0 state) (v rb) (v ll0)))
+    v (gstate_get_n h state) + (v ll - v ll0) / v size_block <= max_size_t /\
+    v (gstate_get_n h state) * (v size_block) + v ll < pow2 128)
+  (ensures  fun h0 _ h1 ->
+    modifies3 state.hash state.block state.n h0 h1 /\
+    state_inv h1 state /\
+    state_eq h1 state (spec_blake2b_incremental_update_inner_longer2 (v ll) h0.[|input|] (spec_of h0 state) (v rb) (v ll0)))
 
-let blake2b_incremental_update_inner_longer2 state ll input rb ll0 =
+let blake2b_incremental_update_inner_longer2 #h state ll input rb ll0 =
   (* Handle all full blocks available *)
+  let n = state_get_n state in
   let n1 = (ll -. ll0) /. size_block in
   let input1 = sub input ll0 (n1 *! size_block) in
   blake2b_incremental_update_loop state n1 input1;
-  {state with n = state.n +! n1;}
+  upd state.n 0ul (n +! n1)
 
 
 noextract
@@ -366,23 +409,22 @@ val blake2b_incremental_update_inner_longer3:
   -> input:lbuffer uint8 ll
   -> rb:size_t{v rb <= v size_block}
   -> ll0:size_t{v ll0 = (if ll <. rb then v ll else v rb)} ->
-  Stack state_r
+  Stack unit
   (requires fun h ->
-    state_inv h state /\ live h input /\
+    live h input /\
     disjoint state.hash input /\ disjoint state.block input /\
     state_inv h state /\
-    v (state.n *. size_block) + v ll < pow2 128)
-  (ensures  fun h0 rstate h1 ->
-    modifies2 state.hash state.block h0 h1 /\
-    state_inv h1 rstate /\
-    state_inv_trans state rstate /\
-    state_eq h1 rstate (spec_blake2b_incremental_update_inner_longer3 (v ll) h0.[|input|] (spec_of h0 state) (v rb) (v ll0)))
+    v (gstate_get_n h state) * (v size_block) + v ll < pow2 128)
+  (ensures  fun h0 _ h1 ->
+    modifies3 state.hash state.block state.pl h0 h1 /\
+    state_inv h1 state /\
+    state_eq h1 state (spec_blake2b_incremental_update_inner_longer3 (v ll) h0.[|input|] (spec_of h0 state) (v rb) (v ll0)))
 
 let blake2b_incremental_update_inner_longer3 state ll input rb ll0 =
   (* Store the remainder *)
   let ll2 = (ll -. ll0) %. size_block in
   blake2b_incremental_update_end state.block ll ll0 ll2 input;
-  ({state with pl = ll2;})
+  upd state.pl 0ul ll2
 
 
 noextract
@@ -445,28 +487,31 @@ let lemma_equal_spec_blake2b_incremental_update_inner_longer ll input state rb l
 
 inline_for_extraction
 val blake2b_incremental_update_inner_longer:
-    state:state_r
-  -> ll:size_t{v state.n + 1 + (v ll / v size_block) <= max_size_t}
+    #h: mem
+  -> state:state_r
+  -> ll:size_t
   -> input:lbuffer uint8 ll
   -> rb:size_t{v rb <= v size_block}
   -> ll0:size_t{v ll0 = (if ll <. rb then v ll else v rb)} ->
-  Stack state_r
+  Stack unit
   (requires fun h ->
-    state_inv h state /\ live h input /\
+    live h input /\
     disjoint state.hash input /\ disjoint state.block input /\
+    disjoint state.n input /\ disjoint state.pl input /\
     state_inv h state /\
-    v (state.n *. size_block) + v ll < pow2 128)
-  (ensures  fun h0 rstate h1 ->
-    modifies2 state.hash state.block h0 h1 /\
-    state_inv h1 rstate /\
-    state_inv_trans state rstate /\
-    state_eq h1 rstate (spec_blake2b_incremental_update_inner_longer (v ll) h0.[|input|] (spec_of h0 state) (v rb) (v ll0)))
+    v (gstate_get_n h state) + 1 + (v ll / v size_block) <= max_size_t /\
+    v (gstate_get_n h state) * (v size_block) + v ll < pow2 128)
+  (ensures  fun h0 _ h1 ->
+    modifies4 state.hash state.block state.n state.pl h0 h1 /\
+    state_inv h1 state /\
+    state_eq h1 state (spec_blake2b_incremental_update_inner_longer_split (v ll) h0.[|input|] (spec_of h0 state) (v rb) (v ll0)))
 
-let blake2b_incremental_update_inner_longer state ll input rb ll0 =
-  let state = blake2b_incremental_update_inner_longer1 state ll input rb ll0 in
-  let state = blake2b_incremental_update_inner_longer2 state ll input rb ll0 in
-  let state = blake2b_incremental_update_inner_longer3 state ll input rb ll0 in
-  state
+let blake2b_incremental_update_inner_longer #h state ll input rb ll0 =
+  let h0 = ST.get () in
+  blake2b_incremental_update_inner_longer1 #h0 state ll input rb ll0;
+  let h1 = ST.get () in
+  blake2b_incremental_update_inner_longer2 #h1 state ll input rb ll0;
+  blake2b_incremental_update_inner_longer3 state ll input rb ll0
 
 
 noextract
@@ -488,25 +533,35 @@ let spec_blake2b_incremental_update_inner state ll rb ll0 input =
 inline_for_extraction
 val blake2b_incremental_update_inner:
     state:state_r
-  -> ll:size_t{v state.n + 1 + v ll / v size_block <= max_size_t}
-  -> rb:size_t{v rb = v size_block - v state.pl /\ v rb <= v size_block}
-  -> ll0:size_t{v ll0 = (if ll <. rb then v ll else v rb) /\ v state.pl + v ll0 <= v size_block}
+  -> ll:size_t
+  -> rb:size_t
+  -> ll0:size_t{v ll0 = (if ll <. rb then v ll else v rb)}
   -> input:lbuffer uint8 ll ->
-  Stack state_r
+  Stack unit
   (requires fun h ->
-    live h input /\ disjoint state.hash input /\ disjoint state.block input /\
+    live h input /\
+    disjoint state.hash input /\ disjoint state.block input /\
+    disjoint state.n input /\ disjoint state.pl input /\
     state_inv h state /\
-    v (state.n *. size_block) + v ll < pow2 128)
-  (ensures  fun h0 rstate h1 ->
-    modifies2 rstate.hash rstate.block h0 h1 /\
-    state_inv h1 rstate /\
-    state_inv_trans state rstate /\
-    state_eq h1 rstate (spec_blake2b_incremental_update_inner (spec_of h0 state) (v ll) (v rb) (v ll0) h0.[|input|]))
+    v (gstate_get_pl h state) + v ll0 <= v size_block /\
+    v rb = v size_block - v (gstate_get_pl h state) /\ v rb <= v size_block /\
+    v (gstate_get_n h state) + 1 + v ll / v size_block <= max_size_t /\
+    v (gstate_get_n h state) * (v size_block) + v ll < pow2 128)
+  (ensures  fun h0 _ h1 ->
+    modifies4 state.hash state.block state.n state.pl h0 h1 /\
+    state_inv h1 state /\
+    state_eq h1 state (spec_blake2b_incremental_update_inner (spec_of h0 state) (v ll) (v rb) (v ll0) h0.[|input|]))
 
 let blake2b_incremental_update_inner state ll rb ll0 input =
-  if ll <=. rb then ({state with pl = state.pl +! ll0})
+  let h0 = ST.get () in
+  let pl = state_get_pl state in
+  if ll <=. rb then (
+    let ha0 = ST.get () in
+    upd state.pl 0ul (pl +! ll0);
+    let ha1 = ST.get () in
+    modifies1_is_modifies4 state.pl state.hash state.block state.n ha0 ha1)
   else
-    blake2b_incremental_update_inner_longer state ll input rb ll0
+    blake2b_incremental_update_inner_longer #h0 state ll input rb ll0
 
 
 noextract
@@ -523,14 +578,19 @@ let spec_compute_branching_condition state ll =
 val compute_branching_condition:
     #h:mem
   -> state:state_r
-  -> ll:size_t{v state.n + 2 + v ll / v size_block <= max_size_t} ->
-  Tot (b:bool{b == spec_compute_branching_condition (spec_of h state) (v ll) })
+  -> ll:size_t{v (gstate_get_n h state) + 2 + v ll / v size_block <= max_size_t} ->
+  Stack bool
+  (requires fun h ->
+    state_inv h state /\
+    v (gstate_get_n h state) + 2 + v ll / v size_block <= max_size_t)
+  (ensures (fun h0 b h1 -> (h0 == h1 /\ b == spec_compute_branching_condition (spec_of h state) (v ll))))
 
 let compute_branching_condition #h state ll =
   [@inline_let]
   let max = normalize_term (size max_size_t) in
   let nll = ll /. size_block in
-  ll =. 0ul || not (state.n +! nll +! 2ul <=. max)
+  let n: size_t = state_get_n state in
+  ll =. 0ul || not (n +! nll +! 2ul <=. max)
 
 
 noextract
@@ -555,29 +615,33 @@ let spec_blake2b_incremental_update state ll input =
 inline_for_extraction
 val blake2b_incremental_update:
     state:state_r
-  -> ll:size_t{v state.n + 2 + v ll / v size_block <= max_size_t}
+  -> ll:size_t
   -> input:lbuffer uint8 ll ->
-  Stack (option state_r)
+  Stack bool
   (requires fun h ->
-    live h input /\ disjoint state.hash input /\ disjoint state.block input /\
+    live h input /\
+    disjoint state.hash input /\ disjoint state.block input /\
+    disjoint state.n input /\ disjoint state.pl input /\
     state_inv h state /\
-    v (state.n *. size_block) + v ll < pow2 128)
-  (ensures  fun h0 orstate h1 ->
-    modifies2 state.hash state.block h0 h1 /\ (
-    let osstate = (SpecI.blake2_incremental_update Spec.Blake2B h0.[|input|] (spec_of h0 state)) in
-    match orstate, osstate with | _,_ -> True | Some rstate, Some sstate ->
-      (* state_eq h1 rstate sstate *)
-      ((spec_of h1 rstate) == sstate)
-   ))
+    v (gstate_get_n h state) + 2 + v ll / v size_block <= max_size_t /\
+    v (gstate_get_n h state) * (v size_block) + v ll < pow2 128)
+  (ensures  fun h0 b h1 ->
+    state_inv h1 state /\
+    modifies4 state.hash state.block state.n state.pl h0 h1 /\
+    (let osstate = (SpecI.blake2_incremental_update Spec.Blake2B h0.[|input|] (spec_of h0 state)) in
+    match osstate with | None -> b == false | Some sstate -> b == true))// /\ (spec_of h1 state) == sstate))
 
 let blake2b_incremental_update state ll input =
   let h0 = ST.get() in
-  if compute_branching_condition #h0 state ll then None else (
-  let rb = size_block -! state.pl in
-  let ll0 = if ll <. rb then ll else rb in
-  let partial = sub input 0ul ll0 in
-  update_sub state.block state.pl ll0 partial;
-  Some(blake2b_incremental_update_inner state ll rb ll0 input))
+  if compute_branching_condition #h0 state ll then false
+  else (
+    let pl = state_get_pl state in
+    let rb = size_block -! pl in
+    let ll0 = if ll <. rb then ll else rb in
+    let partial = sub input 0ul ll0 in
+    update_sub state.block pl ll0 partial;
+    blake2b_incremental_update_inner state ll rb ll0 input;
+    true)
 
 
 val blake2b_incremental_finish:
@@ -596,13 +660,15 @@ val blake2b_incremental_finish:
 
 let blake2b_incremental_finish nn output state =
   let h0 = ST.get () in
-  let last = sub state.block 0ul state.pl in
-  let n64 = to_u64 state.n in
+  let pl = state_get_pl state  in
+  let last = sub state.block 0ul pl in
+  let n = state_get_n state in
+  let n64 = to_u64 n in
   let size_block64 = to_u64 size_block in
-  let pl64 = to_u64 state.pl in
+  let pl64 = to_u64 pl in
   let prev = to_u128 (n64 *! size_block64 +! pl64) in
   assert(v prev = (spec_of h0 state).SpecI.n * (Spec.Blake2.size_block Spec.Blake2.Blake2B) + (spec_of h0 state).SpecI.pl);
-  blake2b_update_last state.hash prev state.pl last;
+  blake2b_update_last state.hash prev pl last;
   blake2b_finish nn output state.hash
 
 
